<?xml version="1.0" encoding="utf-8"?>
<section xml:id="section-1" xmlns:xi="http://www.w3.org/2001/XInclude">
  <title>My First Section</title>
  <introduction>
    <p>Some words</p>
  </introduction>
  <subsection xml:id="subsection-1">
    <title>Natural numbers and integers</title>
    <axiom xml:id="axiom-peano">
      <statement>
        <p>
          There is a set <m>\N</m>, whose elements are called <term>natural numbers</term>,
          and a function <m>s \colon \N \to \N</m>, satisfying:
          <ol marker="1.">
            <li>
              There is an element <m>1 \in \N</m>.
            </li>
            <li>
              There is no <m>n \in \N</m> such that <m>s(n) = 1</m>.
            </li>
            <li>
              The function <m>s</m> is injective (this means that
              <m>s(n) = s(m)</m> only if <m>n = m</m>).
            </li>
            <li xml:id="axiom-induction">
              <title>Principle of induction</title>
              <p>
                Suppose <m>S \subseteq \N</m> is a subset such that
                <m>1 \in S</m> and if <m>n \in S</m> then <m>n+1 \in S</m>.
                Then <m>S = \N</m>.
              </p>
            </li>
          </ol>
          We call <m>s</m> the <term>successor function</term>. Informally
          think of <m>s(n) = n+1</m>.
        </p>
      </statement>
    </axiom>
    <proposition xml:id="prop-predecessors-are-unique">
      <statement>
        <p>
          If <m>n \in \N</m> and <m>n \ne 1</m>, there is a unique <m>m \in \N</m>
          such that <m>s(m) = n</m>.
        </p>
      </statement>
      <proof>
        <p>
          Let <m>
            A = \{ n \in \N : n = 1 or n = s(m)\text{ for some }m \in N \}
            \subseteq \N
          </m>. Then <m>1 \in A</m> and if <m>n \in A</m>, then <m>s(n) \in A</m>,
          so <m>A = \N</m> by <xref ref="axiom-induction"/>. Hence, if <m>n \in \N</m>
          and <m>n \ne 1</m>, then <me>n = s(m)</me> for some <m>m \in \N</m>, which is
          unique since <m>s</m> is injective. Indeed, if <m>n = s(m')</m>, then
          <m>s(m) = s(m')</m>, therefore <me>m = m'</me>.
        </p>
      </proof>
    </proposition>
    <remark>
      <p>
        We set <m>2 = s(1)</m>, <m>3 = s(2)</m>, and so on, so that <m>\N = \{ 1, 2, 3, \ldots \}</m>.
      </p>
    </remark>
    <definition xml:id="def-addition">
      <statement>
        <p>
          We define a binary operation <m>+ \colon \N \times \N \to \N</m> by
          <ol marker="1.">
            <li>For all <m>n \in \N</m>, <m>n + 1 = s(n)</m>.</li>
            <li>For all <m>n, m \in N</m>, <m>n + s(m) = s(n + m)</m>.</li>
          </ol>
        </p>
      </statement>
    </definition>
    <p>
      Observe that this is a recursive definition: <md>
        <mrow>n+1 \amp = s(n)</mrow>
        <mrow>n+2 \amp = n + s(1) = s(n+1) = s(s(n))</mrow>
        <mrow>n+3 \amp = n + s(2) = s(n+2) = s(n + s(1)) = s(s(n + 1)) = s(s(s(n)))</mrow>
      </md>
    </p>
    <proposition xml:id="prop-addition-associative">
      <statement>
        <p>
          For all <m>a, b, c \in \N</m>, we have <me>(a + b) + c = a + (b + c)</me>.
        </p>
      </statement>
      <proof>
        <p>
          Let <m>A = \{ c \in \N \colon (a + b) + c = a + (b + c)\text{ for all }a, b \in \N\}</m>. We
          will show that <m>A = \N</m> using induction <xref ref="axiom-induction"/>. Indeed, for
          <m>a, b \in \N</m>, we have
          <me>(a + b) + 1  = s(a + b) = a + s(b) = a + (b + 1)</me>,
          so <m>1 \in A</m>. Now suppose <m>c \in A</m>. Then for <m>a, b \in \N</m>, we have
          <md>
            <mrow>(a + b) + s(c) \amp = s((a + b) + c) = s(a + (b + c))</mrow>
            <mrow> \amp = a + s(b + c) = a + (b + s(c))</mrow>
          </md>. This shows <m>s(c) \in A</m> and the proof by induction is complete.
        </p>
      </proof>
    </proposition>
    <definition xml:id="def-multiplication">
      <statement>
        <p>
          We define another operation <m>\cdot \colon \N \times \N \to \N</m> by:
          <ol marker="1.">
            <li>
              <p>
                For all <m>n \in \N</m>, <m>n \cdot 1 = n</m>.
              </p>
            </li>
            <li>
              <p>
                For all <m>n, m \in \N</m>, <m>n \cdot s(m) = n \cdot m + n</m>.
              </p>
            </li>
          </ol>
        </p>
      </statement>
    </definition>
    <p>
      Explicitly, <md>
        <mrow>n \cdot 2 \amp = n \cdot s(1) = n \cdot 1 + n = n + n</mrow>
        <mrow>n \cdot 3 \amp = n \cdot s(2) = n \cdot 2 + n = (n + n) + n</mrow>
      </md> and so on.
    </p>
    <proposition xml:id="prop-more-field-axioms">
      <statement>
        <p>
          Let <m>a, b, c \in \N</m>.
        </p>
        <ol>
          <li>
            <p>
              <m>a + b = b + a</m>
            </p>
          </li>
          <li>
            <p>
              If <m>a + c = b + c</m>, then <m>a = b</m>.
            </p>
          </li>
          <li>
            <p>
              <m>a \cdot b = b \cdot a</m>.
            </p>
          </li>
          <li>
            <p>
              <m>a \cdot (b \cdot c) = (a \cdot b) \cdot c</m>.
            </p>
          </li>
          <li>
            <p>
              <m>a \cdot (b + c) = a \cdot b + a \cdot c</m>.
            </p>
          </li>
          <li>
            <p>
              If <m>a \cdot c = b \cdot c</m>, then <m>a = c</m>.
            </p>
          </li>
        </ol>
      </statement>
    </proposition>
    <proof>
      <p>
        Proof of item 5 only. Let
        <me>
          A = \{ c \in \N : a \cdot (b + c) = a \cdot b + a \cdot c \text{ for all } a, b \in \N \}
        </me>. For <m>a, b \in \N</m>, we have
        <me>
          a \cdot (b + 1) = a \cdot s(b) = a \cdot b + a = a\cdot b + a\cdot 1
        </me>, so <m>1 \in A</m>.
      </p>
      <p>
        Now suppose <m>c \in A</m> and let <m>a, b \in \N</m>, so that <m>a \cdot (b+c) = a\cdot b + a \cdot c</m>.
        Then <md>
          <mrow>a \cdot (b + s(c)) \amp = a \cdot s(b + c) = a \cdot (b + c) + a</mrow>
          <mrow>\amp = (a\cdot b + a\cdot c) + a = a\cdot b + a \cdot c + a</mrow>
          <mrow>\amp = a\cdot b + (a\cdot c + a\cdot 1 )= a\cdot b + a(c \cdot 1) = a \cdot b + a\cdot s(c)</mrow>
        </md>, which shows <m>s(c) \in A</m> so that <m>A = \N</m>.
      </p>
    </proof>
    <p>
      Now we give the <term>standard form of induction</term>. Let <m>P(n)</m> be a statement about a
      natural number <m>n</m> that is either true or false. If <m>P(1)</m> is true and if, whenever
      <m>P(n)</m> is true we also have <m>P(n+1)</m> is true, then <m>P(n)</m> is true for all <m>n \in \N</m>.
    </p>
    <definition xml:id="def-less-than">
      <statement>
        <p>
          If <m>m, n \in \N</m>, we say <m>m</m> is <term>less than</term> <m>n</m>, and write <m>m \lt n</m>,
          if <m>n = m + k</m> for some <m>k \in \N</m>. We write <m>m \leq n</m> if we only wish to assert that
          <m>m \lt n</m> or <m>m = n</m>.
        </p>
      </statement>
    </definition>
    <proposition xml:id="prop-order-axioms">
      <statement>
        <p>
          Let <m>a, b, c \in \N</m>.
          <ol>
            <li>
              <p>
                We have <m>a \leq a</m>, but <m>a \not\lt a</m>.
              </p>
            </li>
            <li>
              <p>
                If <m>a \lt b</m> and <m>b \lt c</m>, then <m>a \lt c</m>, and similarly for <m>\leq</m>.
              </p>
            </li>
            <li>
              <p>
                If <m>a \leq b</m> and <m>b \leq a</m>, then <m>a = b</m>.
              </p>
            </li>
            <li>
              <p>
                Exactly one of <m>a \lt b</m> or <m>a = b</m> or <m>b \lt a</m> is true.
              </p>
            </li>
            <li>
              <p>
                We have <m>a \lt b</m> if and only if <m>a + c \lt b + c</m>.
              </p>
            </li>
            <li>
              <p>
                We have <m>a \lt b</m> if and only if <m>a \cdot c \lt b \cdot c</m>.
              </p>
            </li>
          </ol>
        </p>
      </statement>
      <proof>
        <p>
          Proof of 2. Suppose that <m>a \lt b</m> and <m>b \lt c</m>. Then we have
          <m>b = a + k</m> and <m>c = b + \ell</m> for some <m>k, \ell \in \N</m>.
          Then <me>
            c = b + \ell = (a + k) + \ell = a + (k + \ell)
          </me> with <m>k + \ell \in \N</m>, so <m>a \lt c</m>.
        </p>
        <p>
          Proof of 4. First we will show that no more than one of the statements <md>
            <mrow>a \amp \lt b</mrow>
            <mrow>a \amp = b</mrow>
            <mrow>b \amp \lt a</mrow>
          </md> is true. Suppose first that <m>a \lt b</m>. Then <m>b = a + k</m> for
          some <m>k \in \N</m>. Using the fact that <m>m \ne m + n</m> for all <m>m, n \in \N</m>,
          we find <m>b = a + k \ne a</m>. Similarly, if <m>b \lt a</m> then <m>a \ne b</m>.
        </p>
        <p>
          Now if <m>a \lt b</m> and <m>b \lt a</m> then <m>b = a + k</m> and <m>a = b + \ell</m>
          for some <m>k, \ell \in \N</m>, so <me>
            b = (b + \ell) + k = b + (\ell + k)
          </me>, but this implies <m>b \ne b</m>, a contradiction. Similarly, if <m>a = b</m>,
          then <m>a \not\lt b</m> and <m>b \not\lt a</m>. This shows at most one of the statements
          is true.
        </p>
        <p>
          To show at most one of the statements is true, let's fix <m>a \in \N</m> and let
          <m>P(b)</m> be the statement <q><m>a \lt b</m> or <m>a = b</m> or <m>b \lt a</m></q>.
          If <m>a \ne 1</m>, then <m>a = s(k) = 1 + k</m> for some <m>k \in \N</m>, so <m>1 \lt a</m>
          and we have established <m>P(1)</m>. Now, let's suppose that <m>b \in \N</m> and that
          <m>P(b)</m> is true, meaning that <m>a \lt b</m> or <m>a = b</m> or <m>b \lt a</m>.
        </p>
        <p>
          Suppose first that <m>a \lt b</m>. Then <m>b = a + k </m> for some <m>k \in \N</m>,
          so <m>s(b) = s(a+k) = a + s(k)</m>. This shows that <m>a \lt s(b)</m>, so <m>P(b+1)</m>
          is true in this case.
        </p>
        <p>
          Suppose next that <m>a = b</m>. Then <m>s(b) = b + 1 = a + 1</m>, so <m>a \lt s(b)</m>
          and <m>P(b+1)</m> is true as before.
        </p>
        <p>
          Finally, suppose that <m>b \lt a</m>. Then <m>a = b + k</m> for some <m>k</m>. If
          <m>k = 1</m>, then <m>a = b + 1 = s(b)</m>, so <m>P(b+1)</m> is true. If <m>k \ne 1</m>,
          then <m>k = s(\ell)</m> for some <m>\ell \in \N</m> and <me>
            a = b + s(\ell) = b + \ell + 1 = (b + 1) + \ell = s(b) + \ell
          </me>. This shows that <m>a \lt s(b)</m>, and therefore <m>P(b+1)</m> is true in this
          case as well.
        </p>
        <p>
          We have shown that <m>P(b) \implies P(b+1)</m> for all <m>b\in \N</m>, which concludes
          the proof by induction.
        </p>
      </proof>
    </proposition>
    <theorem xml:id="thm-well-ordering">
      <title>The well-ordering principle</title>
      <statement>
        <p>
          If <m>A \subseteq \N</m> is nonempty, then <m>A</m> has a <term>least element</term>.
          That is, there exists <m>a \in A</m> such that <m>a \leq b</m> for all <m>b \in A</m>.
        </p>
      </statement>
    </theorem>

  </subsection>

</section>
